Simplify definition of Reactor (Part 6)

src/ReactorModel/Objects/Reactor/Proper.lean
@@ -1,10 +1,9 @@
 import ReactorModel.Objects.Reactor.Raw
 import ReactorModel.Objects.Reactor.TypeClasses.Proper
 
-open ReactorType in
 structure Reactor where
   raw : Reactor.Raw
-  wf  : Wellformed raw
+  wf  : ReactorType.Wellformed raw
 
 namespace Reactor
 
@@ -24,6 +23,17 @@ instance : ReactorType Reactor where
 instance : ReactorType.Extensional.LawfulCoe Reactor Reactor.Raw where
   coe := Reactor.raw
   coe_ext_iff := by intro (mk ..) (mk ..); simp
+
+theorem wellformed (rtr : Reactor) : ReactorType.Wellformed rtr :=
+  rtr.wf.lift (rtr := rtr)
+
+-- We add these definitions so that we can use dot-notation on `Reactor`s later. Type classes don't
+-- support this notation yet.
+abbrev ports (rtr : Reactor) := ReactorType.ports rtr
+abbrev acts  (rtr : Reactor) := ReactorType.acts rtr
+abbrev state (rtr : Reactor) := ReactorType.state rtr
+abbrev rcns  (rtr : Reactor) := ReactorType.rcns rtr
+abbrev nest  (rtr : Reactor) := ReactorType.nest rtr
 
 noncomputable def scheduledTags (rtr : Reactor) : Set Time.Tag := 
   { g | ∃ i a, (rtr[.act][i] = some a) ∧ (g ∈ a.dom) }
