src/ReactorModel/Objects/Reactor/TypeClasses/Proper.lean
@@ -1,76 +1,162 @@
 import ReactorModel.Objects.Reactor.TypeClasses.Indexable
 
-open ReactorType
+namespace ReactorType
+
 open Indexable
 
 -- About the `↔`-condition in `prio`:  We want to establish a dependency between mutations with 
--- priorities  as well normal reactions with priorities, but not between normal reactions and
+-- priorities as well normal reactions with priorities, but not between normal reactions and
 -- mutations. Otherwise a normal reaction might take precedence over a mutation. Also the precedence
--- of mutations over normal reactions is handled by `mutNorm` - so this would potentially just 
--- create  a redundancy.
+-- of mutations over normal reactions is handled by `mutNorm`, so this would potentially create a
+-- redundancy.
 inductive Dependency [Indexable α] (rtr : α) : ID → ID → Prop
   | prio :
-    (rtr[.rcn][i₁]& = rtr[.rcn][i₂]&) → (rtr[.rcn][i₁] = some rcn₁) → 
-    (rtr[.rcn][i₂] = some rcn₂) → (rcn₁.Mutates ↔ rcn₂.Mutates) → (rcn₁.prio > rcn₂.prio) → 
-    Dependency rtr i₁ i₂
+    (rtr[.rtr][i] = some con) → (rcns con i₁ = some rcn₁) → (rcns con i₂ = some rcn₂) → 
+    (rcn₁.Mutates ↔ rcn₂.Mutates) → (rcn₁.prio > rcn₂.prio) → Dependency rtr i₁ i₂
   | mutNorm : 
-    (rtr[.rcn][iₘ]& = rtr[.rcn][iₙ]&) → (rtr[.rcn][iₘ] = some m) → (rtr[.rcn][iₙ] = some n) →
-    (m.Mutates) → (n.Normal) → Dependency rtr iₘ iₙ
+    (rtr[.rtr][i] = some con) → (rcns con iₘ = some m) → (rcns con iₙ = some n) → (m.Mutates) → 
+    (n.Normal) → Dependency rtr iₘ iₙ
   | depOverlap :
     (rtr[.rcn][i₁] = some rcn₁) → (rtr[.rcn][i₂] = some rcn₂) →
     (rcn₁.deps .out ∩ rcn₂.deps .in).Nonempty → Dependency rtr i₁ i₂
   | mutNest :
-    (rtr[.rcn][iₘ] = some m) → (m.Mutates) → (rtr[.rcn][iₘ]& = some rtr₁) →
-    (nest rtr₁.obj j = some rtr₂) → (iᵣ ∈ (rcns rtr₂).ids) → Dependency rtr iₘ iᵣ
+    (rtr[.rtr][i] = some rtr₁) → (nest rtr₁ j = some rtr₂) → (rcns rtr₁ iₘ = some m) → (m.Mutates) →
+    (iᵣ ∈ (rcns rtr₂).ids) → Dependency rtr iₘ iᵣ
   | trans : 
     Dependency rtr i₁ i₂ → Dependency rtr i₂ i₃ → Dependency rtr i₁ i₃
 
-def Dependency.Acyclic [Indexable α] (rtr : α) : Prop :=
+namespace Dependency
+
+theorem nested [Indexable α] {rtr₁ : α} 
+    (h : nest rtr₁ i = some rtr₂) (d : Dependency rtr₂ i₁ i₂) : Dependency rtr₁ i₁ i₂ := by
+  induction d with
+  | prio h₁          => exact prio (obj?_nested' h h₁).choose_spec ‹_› ‹_› ‹_› ‹_›
+  | mutNorm h₁       => exact mutNorm (obj?_nested' h h₁).choose_spec ‹_› ‹_› ‹_› ‹_›
+  | depOverlap h₁ h₂ => exact depOverlap (obj?_nested h h₁) (obj?_nested h h₂) ‹_›
+  | mutNest h₁       => exact mutNest (obj?_nested' h h₁).choose_spec ‹_› ‹_› ‹_› ‹_›
+  | trans _ _ d₁ d₂  => exact trans d₁ d₂
+
+theorem lower [Indexable α] [Indexable β] [c : ReactorType.LawfulCoe α β] {rtr : α} 
+    (d : Dependency rtr i₁ i₂) : Dependency (rtr : β) i₁ i₂ := by
+  induction d with
+  | prio h₁ h₂ h₃ =>
+     exact prio (c.lower_obj?_some h₁) (c.lower_cmp?_eq_some .rcn h₂) (c.lower_cmp?_eq_some .rcn h₃) 
+           ‹_› ‹_›
+  | mutNorm h₁ h₂ h₃ => 
+    exact mutNorm (c.lower_obj?_some h₁) (c.lower_cmp?_eq_some .rcn h₂)
+          (c.lower_cmp?_eq_some .rcn h₃) ‹_› ‹_›
+  | depOverlap h₁ h₂ => 
+    exact depOverlap (c.lower_obj?_some h₁) (c.lower_obj?_some h₂) ‹_›
+  | mutNest h₁ h₂ h₃ _ h₄ => 
+    exact mutNest (c.lower_obj?_some h₁) (c.lower_cmp?_eq_some .rtr h₂)
+          (c.lower_cmp?_eq_some .rcn h₃) ‹_› (c.lower_mem_cmp?_ids .rcn h₄) 
+  | trans _ _ d₁ d₂ => 
+    exact trans d₁ d₂
+
+def Acyclic [Indexable α] (rtr : α) : Prop :=
   ∀ i, ¬Dependency rtr i i 
 
-variable [Indexable α]
+theorem Acyclic.nested [Indexable α] {rtr₁ : α} 
+    (a : Acyclic rtr₁) (h : nest rtr₁ i = some rtr₂) : Acyclic rtr₂ :=
+  fun i d => absurd (d.nested h) (a i)
 
-theorem Dependency.Acyclic.nested {rtr₁ : α} (a : Acyclic rtr₁) (h : nest rtr₁ i = some rtr₂) : 
-    Acyclic rtr₂ :=
-  sorry
+theorem Acyclic.lift [Indexable α] [Indexable β] [ReactorType.LawfulCoe α β] {rtr : α} 
+    (a : Acyclic (rtr : β)) : Acyclic rtr :=
+  fun i d => absurd d.lower (a i) 
+  
+end Dependency
 
-namespace ReactorType
 namespace Wellformed
 
-inductive NormalDependency (rtr : α) (i : ID) (k : Kind) : Prop
+inductive NormalDependency [ReactorType α] (rtr : α) (i : ID) (k : Kind) : Prop
   | act  (h : i ∈ (acts rtr).ids)
   | prt  (h : ports rtr i = some ⟨v, k⟩)
   | nest (c : nest rtr j = some con) (h : ports con i = some ⟨v, k.opposite⟩)
 
-inductive MutationDependency (rtr : α) (i : ID) : Kind → Prop
+inductive MutationDependency [ReactorType α] (rtr : α) (i : ID) : Kind → Prop
   | act  : (i ∈ (acts rtr).ids)                                    → MutationDependency rtr i k
   | prt  : (ports rtr i = some ⟨v, k⟩)                             → MutationDependency rtr i k
   | nest : (nest rtr j = some con) → (ports con i = some ⟨v, .in⟩) → MutationDependency rtr i .out
 
-structure _root_.ReactorType.Wellformed (rtr : α) : Prop where
-  uniqueInputs : (rtr[.rcn][i₁] = some rcn₁) → (rtr[.rcn][i₂] = some rcn₂) → (i₁ ≠ i₂) → (rtr[.prt][i] = some ⟨v, .in⟩) → (i ∈ rcn₁.deps .out) → (i ∉ rcn₂.deps .out)  
-  overlapPrio  : (rtr[.rtr][i] = some con) → (rcns con i₁ = some rcn₁) → (rcns con i₂ = some rcn₂) → (i₁ ≠ i₂) → (rcn₁.deps .out ∩ rcn₂.deps .out).Nonempty → (rcn₁.prio < rcn₂.prio ∨ rcn₂.prio < rcn₁.prio)
-  impurePrio   : (rtr[.rtr][i] = some con) → (rcns con i₁ = some rcn₁) → (rcns con i₂ = some rcn₂) → (i₁ ≠ i₂) → (¬rcn₁.Pure) → (¬rcn₂.Pure)                → (rcn₁.prio < rcn₂.prio ∨ rcn₂.prio < rcn₁.prio)
-  mutationPrio : (rtr[.rtr][i] = some con) → (rcns con i₁ = some rcn₁) → (rcns con i₂ = some rcn₂) → (i₁ ≠ i₂) → (rcn₁.Mutates) → (rcn₂.Mutates)            → (rcn₁.prio < rcn₂.prio ∨ rcn₂.prio < rcn₁.prio)
-  normalDeps   : (rtr[.rtr][i] = some con) → (rcns con j = some rcn) → (rcn.Normal)  → (d ∈ rcn.deps k) → (NormalDependency con d k) 
-  mutationDeps : (rtr[.rtr][i] = some con) → (rcns con j = some rcn) → (rcn.Mutates) → (d ∈ rcn.deps k) → (MutationDependency con d k) 
+set_option hygiene false in
+scoped macro "norm_and_mut_lift_proof" : term => `(
+  open ReactorType LawfulCoe in
+  fun
+  | act h => .act $ lift_mem_cmp?_ids .act h
+  | prt h => .prt $ lift_cmp?_eq_some .prt h
+  | nest hc hp => by 
+    have h := nest' (rtr := rtr) (β := β) ▸ hc 
+    simp [Partial.map_val] at h
+    obtain ⟨_, _, h⟩ := h
+    subst h
+    exact .nest (lift_cmp?_eq_some .rtr hc) (lift_cmp?_eq_some .prt hp)
+)
+
+theorem NormalDependency.lift 
+    [ReactorType α] [ReactorType β] [ReactorType.LawfulCoe α β] {rtr : α} : 
+    (NormalDependency (rtr : β) i k) → NormalDependency rtr i k :=
+  norm_and_mut_lift_proof
+
+theorem MutationDependency.lift 
+    [ReactorType α] [ReactorType β] [ReactorType.LawfulCoe α β] {rtr : α} :
+    (MutationDependency (rtr : β) i k) → MutationDependency rtr i k :=
+  norm_and_mut_lift_proof
+
+structure _root_.ReactorType.Wellformed [Indexable α] (rtr : α) : Prop where
+  uniqueInputs : (rtr[.rcn][i₁] = some rcn₁) → (rtr[.rcn][i₂] = some rcn₂) → (i₁ ≠ i₂) → 
+                 (rtr[.prt][i] = some ⟨v, .in⟩) → (i ∈ rcn₁.deps .out) → (i ∉ rcn₂.deps .out)  
+  overlapPrio  : (rtr[.rtr][i] = some con) → (rcns con i₁ = some rcn₁) → (rcns con i₂ = some rcn₂) → 
+                 (i₁ ≠ i₂) → (rcn₁.deps .out ∩ rcn₂.deps .out).Nonempty → 
+                 (rcn₁.prio < rcn₂.prio ∨ rcn₂.prio < rcn₁.prio)
+  impurePrio   : (rtr[.rtr][i] = some con) → (rcns con i₁ = some rcn₁) → (rcns con i₂ = some rcn₂) → 
+                 (i₁ ≠ i₂) → (¬rcn₁.Pure) → (¬rcn₂.Pure) → 
+                 (rcn₁.prio < rcn₂.prio ∨ rcn₂.prio < rcn₁.prio)
+  mutationPrio : (rtr[.rtr][i] = some con) → (rcns con i₁ = some rcn₁) → (rcns con i₂ = some rcn₂) → 
+                 (i₁ ≠ i₂) → (rcn₁.Mutates) → (rcn₂.Mutates) →
+                 (rcn₁.prio < rcn₂.prio ∨ rcn₂.prio < rcn₁.prio)
+  normalDeps   : (rtr[.rtr][i] = some con) → (rcns con j = some rcn) → (rcn.Normal) → 
+                 (d ∈ rcn.deps k) → (NormalDependency con d k) 
+  mutationDeps : (rtr[.rtr][i] = some con) → (rcns con j = some rcn) → (rcn.Mutates) →
+                 (d ∈ rcn.deps k) → (MutationDependency con d k) 
   acyclicDeps  : Dependency.Acyclic rtr
 
 set_option hygiene false in
 scoped macro "wf_nested_proof " name:ident : term => `(
   @fun
-  | .nest _ => ($name ‹_› $ obj?_lift h ·)
-  | .root   => ($name ‹_› <| obj?_lift_root h · |>.choose_spec)
+  | .nest _ => ($name ‹_› $ obj?_nested h ·)
+  | .root   => ($name ‹_› <| obj?_nested_root h · |>.choose_spec)
 )
 
-theorem nested {rtr₁ : α} (wf : Wellformed rtr₁) (h : nest rtr₁ i = some rtr₂) : Wellformed rtr₂ where
-  uniqueInputs h₁ h₂ h₃ h₄ := wf.uniqueInputs (obj?_lift h h₁) (obj?_lift h h₂) h₃ (obj?_lift h h₄) 
+theorem nested [Indexable α] {rtr₁ : α} 
+    (wf : Wellformed rtr₁) (h : nest rtr₁ i = some rtr₂) : Wellformed rtr₂ where
   overlapPrio              := wf_nested_proof overlapPrio
   impurePrio               := wf_nested_proof impurePrio
   mutationPrio             := wf_nested_proof mutationPrio
   normalDeps               := wf_nested_proof normalDeps
   mutationDeps             := wf_nested_proof mutationDeps
   acyclicDeps              := wf.acyclicDeps.nested h
+  uniqueInputs h₁ h₂ h₃ h₄ := 
+    wf.uniqueInputs (obj?_nested h h₁) (obj?_nested h h₂) h₃ (obj?_nested h h₄) 
+
+theorem lift [Indexable α] [Indexable β] [c : ReactorType.LawfulCoe α β] {rtr : α} 
+    (wf : Wellformed (rtr : β)) : Wellformed rtr where
+  uniqueInputs h₁ h₂ h₃ h₄ := 
+    wf.uniqueInputs (c.lower_obj?_some h₁) (c.lower_obj?_some h₂) h₃ (c.lower_obj?_some h₄)
+  overlapPrio h₁ h₂ h₃ := 
+    wf.overlapPrio (c.lower_obj?_some h₁) (c.lower_cmp?_eq_some .rcn h₂) 
+    (c.lower_cmp?_eq_some .rcn h₃)
+  impurePrio h₁ h₂ h₃ := 
+    wf.impurePrio (c.lower_obj?_some h₁) (c.lower_cmp?_eq_some .rcn h₂) 
+    (c.lower_cmp?_eq_some .rcn h₃)
+  mutationPrio h₁ h₂ h₃ := 
+    wf.mutationPrio (c.lower_obj?_some h₁) (c.lower_cmp?_eq_some .rcn h₂) 
+    (c.lower_cmp?_eq_some .rcn h₃)
+  normalDeps h₁ h₂ h₃ h₄ := 
+    wf.normalDeps (c.lower_obj?_some h₁) (c.lower_cmp?_eq_some .rcn h₂) h₃ h₄ |>.lift
+  mutationDeps h₁ h₂ h₃ h₄ := 
+    wf.mutationDeps (c.lower_obj?_some h₁) (c.lower_cmp?_eq_some .rcn h₂) h₃ h₄ |>.lift
+  acyclicDeps := 
+    wf.acyclicDeps.lift (rtr := rtr)
 
 end Wellformed
 end ReactorType
